src/Std/Data/HashSet/RawLemmas.lean
@@ -390,6 +390,39 @@ theorem distinct_toList [EquivBEq α] [LawfulHashable α] (h : m.WF) :
     m.toList.Pairwise (fun a b => (a == b) = false) :=
   HashMap.Raw.distinct_keys h.1
 
+section monadic
+
+variable {m : Raw α} {δ : Type v} {m' : Type v → Type v}
+
+theorem foldM_eq_foldlM_toList [Monad m'] [LawfulMonad m'] (h : m.WF)
+    {f : δ → α → m' δ} {init : δ} :
+    m.foldM f init = m.toList.foldlM f init :=
+  HashMap.Raw.foldM_eq_foldlM_keys h.out
+
+theorem fold_eq_foldl_toList (h : m.WF) {f : δ → α → δ} {init : δ} :
+    m.fold f init = m.toList.foldl f init :=
+  HashMap.Raw.fold_eq_foldl_keys h.out
+
+theorem foldRevM_eq_foldrM_toList [Monad m'] [LawfulMonad m'] (h : m.WF)
+    {f : δ → (a : α) → m' δ} {init : δ} :
+    m.foldRevM f init = m.toList.foldrM (fun a b => f b a) init :=
+  HashMap.Raw.foldRevM_eq_foldrM_keys h.out
+
+theorem foldRev_eq_foldr_toList (h : m.WF) {f : δ → (a : α) → δ} {init : δ} :
+    m.foldRev f init = m.toList.foldr (fun a b => f b a) init :=
+  HashMap.Raw.foldRev_eq_foldr_keys h.out
+
+theorem forM_eq_forM_toList [Monad m'] [LawfulMonad m'] (h : m.WF) {f : α → m' PUnit} :
+    m.forM f = m.toList.forM f :=
+  HashMap.Raw.forM_eq_forM_keys h.out
+
+theorem forIn_eq_forIn_toList [Monad m'] [LawfulMonad m'] (h : m.WF)
+    {f : α → δ → m' (ForInStep δ)} {init : δ} :
+    m.forIn f init = ForIn.forIn m.toList init f :=
+  HashMap.Raw.forIn_eq_forIn_keys h.out
+
+end monadic
+
 @[simp]
 theorem insertMany_nil (h : m.WF) :
     insertMany m [] = m :=
